arith/ArithS.lean
@@ -35,6 +35,7 @@ import ArithS.Instance
 import ArithS.InstanceV
 import ArithS.Transparency
 import ArithS.Assembly.Prep
+import ArithS.Assembly.Uniform
 import ArithS.Neg
 import ArithS.Agent
 import ArithS.AgentConverse
